examples/bug-reports/bug111.fst
@@ -1,5 +1,5 @@
 module Bug111
 
-type post (a:Type) = a -> Type
-assume type recv_t: a:Type -> (a -> Type) -> Type
+type post (a:Type) = a -> prop
+assume type recv_t: a:Type -> (a -> prop) -> prop
 assume val recv: unit -> PURE 'a (fun (p:post 'a) -> recv_t 'a p)
