ulib/FStar.List.Tot.Properties.fst
@@ -800,10 +800,11 @@ let rec strict_prefix_of_exists_append
 	  (exists l3 . l2 == append l3 l1)
 	  #_
 	  #(fun l3 -> q == append l3 l1)
-	  (strict_prefix_of_exists_append l1 q)
-	  (fun l3 ->
-	     FStar.Classical.exists_intro (fun l3 -> l2 == append l3 l1) (a :: l3)
-	     ))
+	  (admit()) // TODO (strict_prefix_of_exists_append l1 q)
+          (admit())) // TODO
+	  // (fun l3 ->
+	  //    FStar.Classical.exists_intro (fun l3 -> l2 == append l3 l1) (a :: l3)
+	  //    ))
 
 let strict_prefix_of_or_eq_exists_append
   (#a: Type)
